cancellation/CancelAux2.v
@@ -1,7 +1,7 @@
 Require Import Common.
 Require Import SMod2HMod HMod2Mod Mod2ITree SMod HMod Mod Skeleton.
 Require Import SimGlobal.
-Require Import SMod2HModAux HModInline ElimRel StRed CancelDef.
+Require Import SModCancel HModInline ElimRel StRed CancelDef.
 
 (* Spawn *)
 
@@ -30,7 +30,7 @@ Section CANCEL.
       fn (FIND: alist_find fn (_stb sk0 SKINCL SKWF) = None),
       (<<NONE: stb sk0 fn = None>>).
 
-  Let md_src: HMod.t := SModAux.to_hmod md.
+  Let md_src: HMod.t := SModCancel.to_hmod md.
   Let md_tgt: HMod.t := SMod.to_hmod ginv stb md.
 
   Import CancelTAC.
@@ -65,15 +65,15 @@ Section CANCEL.
               → cid < base.length tgts
               → (∀ (k : nat) (x y : itree modE Any.t), cid ≠ k → srcs !! k = Some x → tgts !! k = Some y → thread_rel ginv stb md sk0 cid k x y)
               → r Any.t Any.t eq ps pt
-                  (x <- interp_stateE Any.t (ITree.iter (handle_schE_callE (ModSem.prog (HModSem.to_mod (HModSemAux.inline (SModSemAux.to_hmod (SMod.modsem md sk0))) rs0))) (cid, srcs)) (Any.pair st rs ↑);; Ret x.2)
-                  (x <- interp_stateE Any.t (ITree.iter (handle_schE_callE (ModSem.prog (HModSem.to_mod (HModSemAux.inline (SModSem.to_hmod (ginv sk0) (stb sk0) (SMod.modsem md sk0))) rt0))) (cid, tgts)) (Any.pair st rt ↑);; Ret x.2))
+                  (x <- interp_stateE Any.t (ITree.iter (handle_schE_callE (ModSem.prog (HModSem.to_mod (HModSemInline.inline (SModSemCancel.to_hmod (SMod.modsem md sk0))) rs0))) (cid, srcs)) (Any.pair st rs ↑);; Ret x.2)
+                  (x <- interp_stateE Any.t (ITree.iter (handle_schE_callE (ModSem.prog (HModSem.to_mod (HModSemInline.inline (SModSem.to_hmod (ginv sk0) (stb sk0) (SMod.modsem md sk0))) rt0))) (cid, tgts)) (Any.pair st rt ↑);; Ret x.2))
   : 
   gpaco7 _simg (cpn7 _simg) bot7 r Any.t Any.t eq ps pt
-  (x <- interp_stateE Any.t (tau;; ITree.iter (handle_schE_callE (ModSem.prog (HModSem.to_mod (HModSemAux.inline (SModSemAux.to_hmod (SMod.modsem md sk0))) rs0)))
+  (x <- interp_stateE Any.t (tau;; ITree.iter (handle_schE_callE (ModSem.prog (HModSem.to_mod (HModSemInline.inline (SModSemCancel.to_hmod (SMod.modsem md sk0))) rs0)))
     (cid, <[cid:=tau;; interp_hp (tau;; trigger (Yield (base.length srcs));;; ktrS (base.length srcs))]> srcs ++ 
             [sem <- (alist_find fn (List.map (map_snd (interp_hp_fun ∘ HModSem.sandbox_body))
-                    (List.map (map_snd (wrap_elimI (SModSemAux.to_hmod (SMod.modsem md sk0))))
-                    (List.map (map_snd (λ ksb : list string * fspecbody, (ksb.1, interp_sb_hp_aux ksb.2))) (SModSem.fnsems (SMod.modsem md sk0)))))) !;; sem args])) (Any.pair st rs ↑);; Ret x.2)
+                    (List.map (map_snd (wrap_elimI (SModSemCancel.to_hmod (SMod.modsem md sk0))))
+                    (List.map (map_snd (λ ksb : list string * fspecbody, (ksb.1, interp_sb_hp_cancel ksb.2))) (SModSem.fnsems (SMod.modsem md sk0)))))) !;; sem args])) (Any.pair st rs ↑);; Ret x.2)
   (x <- interp_stateE Any.t
     (x_ <- trigger (|resum IFun (SMod2HMod.meta f) (Choose (SMod2HMod.meta f)))%sum;;
       x_0 <- Ret (inl
@@ -92,7 +92,7 @@ Section CANCEL.
                    | inr r0 => Ret r0
                    end]> tgts));;
       match x_0 with
-      | inl l0 => tau;; ITree.iter (handle_schE_callE (ModSem.prog (HModSem.to_mod (HModSemAux.inline (SModSem.to_hmod (ginv sk0) (stb sk0) (SMod.modsem md sk0))) rt0))) l0
+      | inl l0 => tau;; ITree.iter (handle_schE_callE (ModSem.prog (HModSem.to_mod (HModSemInline.inline (SModSem.to_hmod (ginv sk0) (stb sk0) (SMod.modsem md sk0))) rt0))) l0
       | inr r0 => Ret r0
       end) (Any.pair st rt ↑);; Ret x.2).
   Proof.
@@ -126,8 +126,8 @@ Section CANCEL.
        [' sem : (Any.t → itree modE Any.t) <-
         (alist_find fn
            (List.map (map_snd (interp_hp_fun ∘ HModSem.sandbox_body))
-              (List.map (map_snd (wrap_elimI (SModSemAux.to_hmod (SMod.modsem md sk0))))
-                 (List.map (map_snd (λ ksb : list string * fspecbody, (ksb.1, interp_sb_hp_aux ksb.2))) (SModSem.fnsems (SMod.modsem md sk0)))))) !;; 
+              (List.map (map_snd (wrap_elimI (SModSemCancel.to_hmod (SMod.modsem md sk0))))
+                 (List.map (map_snd (λ ksb : list string * fspecbody, (ksb.1, interp_sb_hp_cancel ksb.2))) (SModSem.fnsems (SMod.modsem md sk0)))))) !;; 
         sem args])).
     { rewrite length_app. nia. }
     iterT 2.
@@ -138,7 +138,7 @@ Section CANCEL.
     erewrite wrap_elimI_well_scoped; cycle 1.
     {
       instantiate (1:= fn).
-      s. unfold interp_sb_hp_aux. s.
+      s. unfold interp_sb_hp_cancel. s.
       rewrite alist_find_map_snd H1. ss.
     }
     erewrite wrap_elimI_well_scoped; cycle 1.
@@ -149,7 +149,7 @@ Section CANCEL.
     }
     ired.
     unfold interp_hp_fun, inline_hp_fun, HModSem.sandbox_body. s. 
-    unfold interp_sb_hp, interp_sb_hp_aux. s.
+    unfold interp_sb_hp, interp_sb_hp_cancel. s.
     hide_l. _iter.
     rewrite list_lookup_insert_ne; try nia. 
     rewrite list_lookup_length. ired. tau 1.
